TAO_5_Quantifiable.thy
@@ -20,16 +20,18 @@ subsection{* Type Class *}
 
 text{* Datatype for types for which quantification is defined: *}
 
-datatype var = \<nu>var (var\<nu>: \<nu>) | \<o>var (var\<o>: \<o>) | \<Pi>\<^sub>1var (var\<Pi>\<^sub>1: \<Pi>\<^sub>1)
+datatype var = \<kappa>var (var\<kappa>: \<kappa>) | \<o>var (var\<o>: \<o>) | \<Pi>\<^sub>1var (var\<Pi>\<^sub>1: \<Pi>\<^sub>1)
              | \<Pi>\<^sub>2var (var\<Pi>\<^sub>2: \<Pi>\<^sub>2) | \<Pi>\<^sub>3var (var\<Pi>\<^sub>3: \<Pi>\<^sub>3)
 
 text{* Type class for quantifiable types: *}
 
 class quantifiable = fixes forall :: "('a\<Rightarrow>\<o>)\<Rightarrow>\<o>" (binder "\<^bold>\<forall>" [8] 9)
+                       and domain :: "'a set"
                        and qvar :: "'a\<Rightarrow>var"
                        and varq :: "var\<Rightarrow>'a"
-  assumes quantifiable_T8: "(w \<Turnstile> (\<^bold>\<forall> x . \<psi> x)) = (\<forall> x . (w \<Turnstile> (\<psi> x)))"
+  assumes quantifiable_T8: "(w \<Turnstile> (\<^bold>\<forall> x . \<psi> x)) = (\<forall> x . x \<in> domain \<longrightarrow> (w \<Turnstile> (\<psi> x)))"
       and varq_qvar_id: "varq (qvar x) = x"
+      and nonempty: "\<exists> x . x \<in> domain"
 begin
   definition exists :: "('a\<Rightarrow>\<o>)\<Rightarrow>\<o>" (binder "\<^bold>\<exists>" [8] 9) where
     "exists \<equiv> \<lambda> \<phi> . \<^bold>\<not>(\<^bold>\<forall> x . \<^bold>\<not>\<phi> x)"
@@ -38,88 +40,103 @@ end
 
 text{* Semantics for the general all quantifier: *}
 
-lemma (in Semantics) T8: shows "(w \<Turnstile> \<^bold>\<forall> x . \<psi> x) = (\<forall> x . (w \<Turnstile> \<psi> x))"
+lemma (in Semantics) T8: shows "(w \<Turnstile> \<^bold>\<forall> x . \<psi> x) = (\<forall> x . x \<in> domain \<longrightarrow> (w \<Turnstile> \<psi> x))"
   using quantifiable_T8 .
 
 subsection{* Instantiations *}
 
-instantiation \<nu> :: quantifiable
+instantiation \<kappa> :: quantifiable
 begin
-  definition forall_\<nu> :: "(\<nu>\<Rightarrow>\<o>)\<Rightarrow>\<o>" where "forall_\<nu> \<equiv> forall\<^sub>\<nu>"
-  definition qvar_\<nu> :: "\<nu>\<Rightarrow>var" where "qvar \<equiv> \<nu>var"
-  definition varq_\<nu> :: "var\<Rightarrow>\<nu>" where "varq \<equiv> var\<nu>"
+  definition forall_\<kappa> :: "(\<kappa>\<Rightarrow>\<o>)\<Rightarrow>\<o>" where "forall_\<kappa> \<equiv> forall\<^sub>\<nu>"
+  definition domain_\<kappa> :: "\<kappa> set" where "domain_\<kappa> \<equiv> { x . denotes (x)}"
+  definition qvar_\<kappa> :: "\<kappa>\<Rightarrow>var" where "qvar \<equiv> \<kappa>var"
+  definition varq_\<kappa> :: "var\<Rightarrow>\<kappa>" where "varq \<equiv> var\<kappa>"
   instance proof
-    fix w :: i and \<psi> :: "\<nu>\<Rightarrow>\<o>"
-    show "(w \<Turnstile> \<^bold>\<forall>x. \<psi> x) = (\<forall>x. (w \<Turnstile> \<psi> x))"
-      unfolding forall_\<nu>_def using Semantics.T8_\<nu> .
+    fix w :: i and \<psi> :: "\<kappa>\<Rightarrow>\<o>"
+    show "(w \<Turnstile> \<^bold>\<forall>x. \<psi> x) = (\<forall>x. x \<in> domain \<longrightarrow> (w \<Turnstile> \<psi> x))"
+      unfolding forall_\<kappa>_def domain_\<kappa>_def using Semantics.T8_\<nu> by auto
   next
-    fix x :: \<nu>
+    fix x :: \<kappa>
     show "varq (qvar x) = x"
-      unfolding qvar_\<nu>_def varq_\<nu>_def by simp
+      unfolding qvar_\<kappa>_def varq_\<kappa>_def by simp
+  next
+    show "\<exists>x :: \<kappa> . x \<in> domain" unfolding domain_\<kappa>_def unfolding denotes_def apply simp apply transfer by auto
   qed
 end
 
 instantiation \<o> :: quantifiable
 begin
   definition forall_\<o> :: "(\<o>\<Rightarrow>\<o>)\<Rightarrow>\<o>" where "forall_\<o> \<equiv> forall\<^sub>\<o>"
+  definition domain_\<o> :: "\<o> set" where "domain_\<o> \<equiv> UNIV"
   definition qvar_\<o> :: "\<o>\<Rightarrow>var" where "qvar \<equiv> \<o>var"
   definition varq_\<o> :: "var\<Rightarrow>\<o>" where "varq \<equiv> var\<o>"
   instance proof
     fix w :: i and \<psi> :: "\<o>\<Rightarrow>\<o>"
-    show "(w \<Turnstile> \<^bold>\<forall>x. \<psi> x) = (\<forall>x. (w \<Turnstile> \<psi> x))"
-      unfolding forall_\<o>_def using Semantics.T8_\<o> .
+    show "(w \<Turnstile> \<^bold>\<forall>x. \<psi> x) = (\<forall>x. x \<in> domain \<longrightarrow> (w \<Turnstile> \<psi> x))"
+      unfolding forall_\<o>_def domain_\<o>_def using Semantics.T8_\<o> by simp
   next
     fix x :: \<o>
     show "varq (qvar x) = x"
       unfolding qvar_\<o>_def varq_\<o>_def by simp
+  next
+    show "\<exists>x :: \<o> . x \<in> domain" unfolding domain_\<o>_def by auto
   qed
 end
 
 instantiation \<Pi>\<^sub>1 :: quantifiable
 begin
   definition forall_\<Pi>\<^sub>1 :: "(\<Pi>\<^sub>1\<Rightarrow>\<o>)\<Rightarrow>\<o>" where "forall_\<Pi>\<^sub>1 \<equiv> forall\<^sub>1"
+  definition domain_\<Pi>\<^sub>1 :: "\<Pi>\<^sub>1 set" where "domain_\<Pi>\<^sub>1 \<equiv> UNIV"
   definition qvar_\<Pi>\<^sub>1 :: "\<Pi>\<^sub>1\<Rightarrow>var" where "qvar \<equiv> \<Pi>\<^sub>1var"
   definition varq_\<Pi>\<^sub>1 :: "var\<Rightarrow>\<Pi>\<^sub>1" where "varq \<equiv> var\<Pi>\<^sub>1"
   instance proof
     fix w :: i and \<psi> :: "\<Pi>\<^sub>1\<Rightarrow>\<o>"
-    show "(w \<Turnstile> \<^bold>\<forall>x. \<psi> x) = (\<forall>x. (w \<Turnstile> \<psi> x))"
-      unfolding forall_\<Pi>\<^sub>1_def using Semantics.T8_1 .
+    show "(w \<Turnstile> \<^bold>\<forall>x. \<psi> x) = (\<forall>x. x \<in> domain \<longrightarrow> (w \<Turnstile> \<psi> x))"
+      unfolding forall_\<Pi>\<^sub>1_def domain_\<Pi>\<^sub>1_def using Semantics.T8_1 by simp
   next
     fix x :: \<Pi>\<^sub>1
     show "varq (qvar x) = x"
       unfolding qvar_\<Pi>\<^sub>1_def varq_\<Pi>\<^sub>1_def by simp
+  next
+    show "\<exists>x :: \<Pi>\<^sub>1 . x \<in> domain" unfolding domain_\<Pi>\<^sub>1_def by auto
   qed
 end
 
 instantiation \<Pi>\<^sub>2 :: quantifiable
 begin
   definition forall_\<Pi>\<^sub>2 :: "(\<Pi>\<^sub>2\<Rightarrow>\<o>)\<Rightarrow>\<o>" where "forall_\<Pi>\<^sub>2 \<equiv> forall\<^sub>2"
+  definition domain_\<Pi>\<^sub>2 :: "\<Pi>\<^sub>2 set" where "domain_\<Pi>\<^sub>2 \<equiv> UNIV"
   definition qvar_\<Pi>\<^sub>2 :: "\<Pi>\<^sub>2\<Rightarrow>var" where "qvar \<equiv> \<Pi>\<^sub>2var"
   definition varq_\<Pi>\<^sub>2 :: "var\<Rightarrow>\<Pi>\<^sub>2" where "varq \<equiv> var\<Pi>\<^sub>2"
   instance proof
     fix w :: i and \<psi> :: "\<Pi>\<^sub>2\<Rightarrow>\<o>"
-    show "(w \<Turnstile> \<^bold>\<forall>x. \<psi> x) = (\<forall>x. (w \<Turnstile> \<psi> x))"
-      unfolding forall_\<Pi>\<^sub>2_def using Semantics.T8_2 .
+    show "(w \<Turnstile> \<^bold>\<forall>x. \<psi> x) = (\<forall>x. x \<in> domain \<longrightarrow> (w \<Turnstile> \<psi> x))"
+      unfolding forall_\<Pi>\<^sub>2_def domain_\<Pi>\<^sub>2_def using Semantics.T8_2 by simp
   next
     fix x :: \<Pi>\<^sub>2
     show "varq (qvar x) = x"
       unfolding qvar_\<Pi>\<^sub>2_def varq_\<Pi>\<^sub>2_def by simp
+  next
+    show "\<exists>x :: \<Pi>\<^sub>2 . x \<in> domain" unfolding domain_\<Pi>\<^sub>2_def by auto
   qed
 end
 
 instantiation \<Pi>\<^sub>3 :: quantifiable
 begin
   definition forall_\<Pi>\<^sub>3 :: "(\<Pi>\<^sub>3\<Rightarrow>\<o>)\<Rightarrow>\<o>" where "forall_\<Pi>\<^sub>3 \<equiv> forall\<^sub>3"
+  definition domain_\<Pi>\<^sub>3 :: "\<Pi>\<^sub>3 set" where "domain_\<Pi>\<^sub>3 \<equiv> UNIV"
   definition qvar_\<Pi>\<^sub>3 :: "\<Pi>\<^sub>3\<Rightarrow>var" where "qvar \<equiv> \<Pi>\<^sub>3var"
   definition varq_\<Pi>\<^sub>3 :: "var\<Rightarrow>\<Pi>\<^sub>3" where "varq \<equiv> var\<Pi>\<^sub>3"
   instance proof
     fix w :: i and \<psi> :: "\<Pi>\<^sub>3\<Rightarrow>\<o>"
-    show "(w \<Turnstile> \<^bold>\<forall>x. \<psi> x) = (\<forall>x. (w \<Turnstile> \<psi> x))"
-      unfolding forall_\<Pi>\<^sub>3_def using Semantics.T8_3 .
+    show "(w \<Turnstile> \<^bold>\<forall>x. \<psi> x) = (\<forall>x. x \<in> domain \<longrightarrow> (w \<Turnstile> \<psi> x))"
+      unfolding forall_\<Pi>\<^sub>3_def domain_\<Pi>\<^sub>3_def using Semantics.T8_3 by simp
   next
     fix x :: \<Pi>\<^sub>3
     show "varq (qvar x) = x"
       unfolding qvar_\<Pi>\<^sub>3_def varq_\<Pi>\<^sub>3_def by simp
+  next
+    show "\<exists>x :: \<Pi>\<^sub>3 . x \<in> domain" unfolding domain_\<Pi>\<^sub>3_def by auto
   qed
 end
 
@@ -137,19 +154,19 @@ begin
   subsubsection{* Rules for General All Quantification. *}
   lemma AllI[meta_intro]: "(\<And>x::'a::quantifiable. [\<phi> x in v]) \<Longrightarrow> [\<^bold>\<forall> x. \<phi> x in v]"
     by (auto simp: Semantics.T8)
-  lemma AllE[meta_elim]: "[\<^bold>\<forall>x. \<phi> x in v] \<Longrightarrow> (\<And>x::'a::quantifiable.[\<phi> x in v])"
+  lemma AllE[meta_elim]: "[\<^bold>\<forall>x. \<phi> x in v] \<Longrightarrow> (\<And>x::'a::quantifiable. x \<in> domain \<longrightarrow> [\<phi> x in v])"
     by (auto simp: Semantics.T8)
-  lemma AllS[meta_subst]: "[\<^bold>\<forall>x. \<phi> x in v] = (\<forall>x::'a::quantifiable.[\<phi> x in v])"
+  lemma AllS[meta_subst]: "[\<^bold>\<forall>x. \<phi> x in v] = (\<forall>x::'a::quantifiable. x \<in> domain \<longrightarrow> [\<phi> x in v])"
     by (auto simp: Semantics.T8)
 
   subsubsection{* Rules for Existence *}
-  lemma ExIRule: "([\<phi> y in v]) \<Longrightarrow> [\<^bold>\<exists>x. \<phi> x in v]"
+  lemma ExIRule: "(y \<in> domain \<and> [\<phi> y in v]) \<Longrightarrow> [\<^bold>\<exists>x. \<phi> x in v]"
     by (auto simp: exists_def NotS AllS)
-  lemma ExI[meta_intro]: "(\<exists> y . [\<phi> y in v]) \<Longrightarrow> [\<^bold>\<exists>x. \<phi> x in v]"
+  lemma ExI[meta_intro]: "(\<exists> y . y \<in> domain \<and> [\<phi> y in v]) \<Longrightarrow> [\<^bold>\<exists>x. \<phi> x in v]"
     by (auto simp: exists_def NotS AllS)
-  lemma ExE[meta_elim]: "[\<^bold>\<exists>x. \<phi> x in v] \<Longrightarrow> (\<exists> y . [\<phi> y in v])"
+  lemma ExE[meta_elim]: "[\<^bold>\<exists>x. \<phi> x in v] \<Longrightarrow> (\<exists> y .  y \<in> domain \<and>[\<phi> y in v])"
     by (auto simp: exists_def NotS AllS)
-  lemma ExS[meta_subst]: "[\<^bold>\<exists>x. \<phi> x in v] = (\<exists> y . [\<phi> y in v])"
+  lemma ExS[meta_subst]: "[\<^bold>\<exists>x. \<phi> x in v] = (\<exists> y .  y \<in> domain \<and>[\<phi> y in v])"
     by (auto simp: exists_def NotS AllS)
   lemma ExERule: assumes "[\<^bold>\<exists>x. \<phi> x in v]" obtains x where "[\<phi> x in v]" 
     using ExE assms by auto
