TAO_6_Identifiable.thy
@@ -22,6 +22,8 @@ class identifiable =
 fixes identity :: "'a\<Rightarrow>'a\<Rightarrow>\<o>" (infixl "\<^bold>=" 63)
 assumes l_identity:
   "w \<Turnstile> x \<^bold>= y \<Longrightarrow> w \<Turnstile> \<phi> x \<Longrightarrow> w \<Turnstile> \<phi> y"
+assumes meta_identity:
+  "w \<Turnstile> x \<^bold>= y \<Longrightarrow> x = y"
 begin
   abbreviation notequal (infixl "\<^bold>\<noteq>" 63) where
     "notequal \<equiv> \<lambda> x y . \<^bold>\<not>(x \<^bold>= y)"
@@ -45,23 +47,12 @@ begin
     show "[x \<^bold>= y in w] \<Longrightarrow> [\<phi> x in w] \<Longrightarrow> [\<phi> y in w]"
       unfolding identity_\<kappa>_def
       using MetaSolver.Eq\<kappa>_prop ..
-  qed
-end
-
-instantiation \<nu> :: identifiable
-begin
-  definition identity_\<nu> where "identity_\<nu> \<equiv> \<lambda> x y . x\<^sup>P \<^bold>= y\<^sup>P"
-  instance proof
-    fix \<alpha> :: \<nu> and \<beta> :: \<nu> and v \<phi>
-    assume "v \<Turnstile> \<alpha> \<^bold>= \<beta>"
-    hence "v \<Turnstile> \<alpha>\<^sup>P \<^bold>= \<beta>\<^sup>P"
-      unfolding identity_\<nu>_def by auto
-    hence "\<And>\<phi>.(v \<Turnstile> \<phi> (\<alpha>\<^sup>P)) \<Longrightarrow> (v \<Turnstile> \<phi> (\<beta>\<^sup>P))"
-      using l_identity by auto
-    hence "(v \<Turnstile> \<phi> (denotation (\<alpha>\<^sup>P))) \<Longrightarrow> (v \<Turnstile> \<phi> (denotation (\<beta>\<^sup>P)))"
-      by meson
-    thus "(v \<Turnstile> \<phi> \<alpha>) \<Longrightarrow> (v \<Turnstile> \<phi> \<beta>)"
-      by (simp only: proper_denotation)
+  next
+    interpret MetaSolver .
+    fix w :: i and x y :: \<kappa>
+      show "[x \<^bold>= y in w] \<Longrightarrow> x = y" using Eq\<kappa>_prop
+            unfolding identity_\<kappa>_def
+            using MetaSolver.Eq\<kappa>E Semantics.d\<^sub>\<kappa>_inject by blast
   qed
 end
 
@@ -72,6 +63,12 @@ begin
     fix F G :: \<Pi>\<^sub>1 and w \<phi>
     show "(w \<Turnstile> F \<^bold>= G) \<Longrightarrow> (w \<Turnstile> \<phi> F) \<Longrightarrow> (w \<Turnstile> \<phi> G)"
       unfolding identity_\<Pi>\<^sub>1_def using MetaSolver.Eq\<^sub>1_prop ..
+  next
+    interpret MetaSolver .
+    fix w :: i and x y :: \<Pi>\<^sub>1
+      show "[x \<^bold>= y in w] \<Longrightarrow> x = y" using Eq\<kappa>_prop
+            unfolding identity_\<Pi>\<^sub>1_def
+            using MetaSolver.Eq\<^sub>1E Semantics.d\<^sub>\<kappa>_inject by blast
   qed
 end
 
@@ -82,6 +79,12 @@ begin
     fix F G :: \<Pi>\<^sub>2 and w \<phi>
     show "(w \<Turnstile> F \<^bold>= G) \<Longrightarrow> (w \<Turnstile> \<phi> F) \<Longrightarrow> (w \<Turnstile> \<phi> G)"
       unfolding identity_\<Pi>\<^sub>2_def using MetaSolver.Eq\<^sub>2_prop ..
+  next
+    interpret MetaSolver .
+    fix w :: i and x y :: \<Pi>\<^sub>2
+      show "[x \<^bold>= y in w] \<Longrightarrow> x = y" using Eq\<kappa>_prop
+            unfolding identity_\<Pi>\<^sub>2_def
+            using MetaSolver.Eq\<^sub>2E Semantics.d\<^sub>\<kappa>_inject by blast
   qed
 end
 
@@ -92,6 +95,12 @@ begin
     fix F G :: \<Pi>\<^sub>3 and w \<phi>
     show "(w \<Turnstile> F \<^bold>= G) \<Longrightarrow> (w \<Turnstile> \<phi> F) \<Longrightarrow> (w \<Turnstile> \<phi> G)"
       unfolding identity_\<Pi>\<^sub>3_def using MetaSolver.Eq\<^sub>3_prop ..
+  next
+    interpret MetaSolver .
+    fix w :: i and x y :: \<Pi>\<^sub>3
+      show "[x \<^bold>= y in w] \<Longrightarrow> x = y" using Eq\<kappa>_prop
+            unfolding identity_\<Pi>\<^sub>3_def
+            using MetaSolver.Eq\<^sub>3E Semantics.d\<^sub>\<kappa>_inject by blast
   qed
 end
 
@@ -102,10 +111,16 @@ begin
     fix F G :: \<o> and w \<phi>
     show "(w \<Turnstile> F \<^bold>= G) \<Longrightarrow> (w \<Turnstile> \<phi> F) \<Longrightarrow> (w \<Turnstile> \<phi> G)"
       unfolding identity_\<o>_def using MetaSolver.Eq\<^sub>\<o>_prop ..
+  next
+    interpret MetaSolver .
+    fix w :: i and x y :: \<o>
+      show "[x \<^bold>= y in w] \<Longrightarrow> x = y" using Eq\<^sub>\<o>_prop
+            unfolding identity_\<o>_def
+            using MetaSolver.Eq\<^sub>\<o>E Semantics.d\<^sub>\<kappa>_inject by blast
   qed
 end
 
-instance \<nu> :: quantifiable_and_identifiable ..
+instance \<kappa> :: quantifiable_and_identifiable ..
 instance \<Pi>\<^sub>1 :: quantifiable_and_identifiable ..
 instance \<Pi>\<^sub>2 :: quantifiable_and_identifiable ..
 instance \<Pi>\<^sub>3 :: quantifiable_and_identifiable ..
@@ -123,28 +138,25 @@ text{*
 
 named_theorems identity_defs
 lemma identity\<^sub>E_def[identity_defs]:
-  "basic_identity\<^sub>E \<equiv> \<^bold>\<lambda>\<^sup>2 (\<lambda>x y. \<lparr>O!,x\<^sup>P\<rparr> \<^bold>& \<lparr>O!,y\<^sup>P\<rparr> \<^bold>& \<^bold>\<box>(\<^bold>\<forall>F. \<lparr>F,x\<^sup>P\<rparr> \<^bold>\<equiv> \<lparr>F,y\<^sup>P\<rparr>))"
+  "basic_identity\<^sub>E \<equiv> \<^bold>\<lambda>\<^sup>2 (\<lambda>x y. \<lparr>O!,x\<rparr> \<^bold>& \<lparr>O!,y\<rparr> \<^bold>& \<^bold>\<box>(\<^bold>\<forall>F. \<lparr>F,x\<rparr> \<^bold>\<equiv> \<lparr>F,y\<rparr>))"
   unfolding basic_identity\<^sub>E_def forall_\<Pi>\<^sub>1_def by simp
 lemma identity\<^sub>E_infix_def[identity_defs]:
   "x \<^bold>=\<^sub>E y \<equiv> \<lparr>basic_identity\<^sub>E,x,y\<rparr>" using basic_identity\<^sub>E_infix_def .
 lemma identity\<^sub>\<kappa>_def[identity_defs]:
   "op \<^bold>= \<equiv> \<lambda>x y. x \<^bold>=\<^sub>E y \<^bold>\<or> \<lparr>A!,x\<rparr> \<^bold>& \<lparr>A!,y\<rparr> \<^bold>& \<^bold>\<box>(\<^bold>\<forall> F. \<lbrace>x,F\<rbrace> \<^bold>\<equiv> \<lbrace>y,F\<rbrace>)"
   unfolding identity_\<kappa>_def basic_identity\<^sub>\<kappa>_def forall_\<Pi>\<^sub>1_def by simp
-lemma identity\<^sub>\<nu>_def[identity_defs]:
-  "op \<^bold>= \<equiv> \<lambda>x y. (x\<^sup>P) \<^bold>=\<^sub>E (y\<^sup>P) \<^bold>\<or> \<lparr>A!,x\<^sup>P\<rparr> \<^bold>& \<lparr>A!,y\<^sup>P\<rparr> \<^bold>& \<^bold>\<box>(\<^bold>\<forall> F. \<lbrace>x\<^sup>P,F\<rbrace> \<^bold>\<equiv> \<lbrace>y\<^sup>P,F\<rbrace>)"
-  unfolding identity_\<nu>_def identity\<^sub>\<kappa>_def by simp
 lemma identity\<^sub>1_def[identity_defs]:
-  "op \<^bold>= \<equiv> \<lambda>F G. \<^bold>\<box>(\<^bold>\<forall> x . \<lbrace>x\<^sup>P,F\<rbrace> \<^bold>\<equiv> \<lbrace>x\<^sup>P,G\<rbrace>)"
-  unfolding identity_\<Pi>\<^sub>1_def basic_identity\<^sub>1_def forall_\<nu>_def by simp
+  "op \<^bold>= \<equiv> \<lambda>F G. \<^bold>\<box>(\<^bold>\<forall> x . \<lbrace>x,F\<rbrace> \<^bold>\<equiv> \<lbrace>x,G\<rbrace>)"
+  unfolding identity_\<Pi>\<^sub>1_def basic_identity\<^sub>1_def forall_\<kappa>_def by simp
 lemma identity\<^sub>2_def[identity_defs]:
-  "op \<^bold>= \<equiv> \<lambda>F G. \<^bold>\<forall> x. (\<^bold>\<lambda>y. \<lparr>F,x\<^sup>P,y\<^sup>P\<rparr>) \<^bold>= (\<^bold>\<lambda>y. \<lparr>G,x\<^sup>P,y\<^sup>P\<rparr>)
-                    \<^bold>& (\<^bold>\<lambda>y. \<lparr>F,y\<^sup>P,x\<^sup>P\<rparr>) \<^bold>= (\<^bold>\<lambda>y. \<lparr>G,y\<^sup>P,x\<^sup>P\<rparr>)"
-  unfolding identity_\<Pi>\<^sub>2_def identity_\<Pi>\<^sub>1_def basic_identity\<^sub>2_def forall_\<nu>_def by simp
+  "op \<^bold>= \<equiv> \<lambda>F G. \<^bold>\<forall> x. (\<^bold>\<lambda>y. \<lparr>F,x,y\<rparr>) \<^bold>= (\<^bold>\<lambda>y. \<lparr>G,x,y\<rparr>)
+                    \<^bold>& (\<^bold>\<lambda>y. \<lparr>F,y,x\<rparr>) \<^bold>= (\<^bold>\<lambda>y. \<lparr>G,y,x\<rparr>)"
+  unfolding identity_\<Pi>\<^sub>2_def identity_\<Pi>\<^sub>1_def basic_identity\<^sub>2_def forall_\<kappa>_def by simp
 lemma identity\<^sub>3_def[identity_defs]:
-  "op \<^bold>= \<equiv> \<lambda>F G. \<^bold>\<forall> x y. (\<^bold>\<lambda>z. \<lparr>F,z\<^sup>P,x\<^sup>P,y\<^sup>P\<rparr>) \<^bold>= (\<^bold>\<lambda>z. \<lparr>G,z\<^sup>P,x\<^sup>P,y\<^sup>P\<rparr>)
-                      \<^bold>& (\<^bold>\<lambda>z. \<lparr>F,x\<^sup>P,z\<^sup>P,y\<^sup>P\<rparr>) \<^bold>= (\<^bold>\<lambda>z. \<lparr>G,x\<^sup>P,z\<^sup>P,y\<^sup>P\<rparr>)
-                      \<^bold>& (\<^bold>\<lambda>z. \<lparr>F,x\<^sup>P,y\<^sup>P,z\<^sup>P\<rparr>) \<^bold>= (\<^bold>\<lambda>z. \<lparr>G,x\<^sup>P,y\<^sup>P,z\<^sup>P\<rparr>)"
-  unfolding identity_\<Pi>\<^sub>3_def identity_\<Pi>\<^sub>1_def basic_identity\<^sub>3_def forall_\<nu>_def by simp
+  "op \<^bold>= \<equiv> \<lambda>F G. \<^bold>\<forall> x y. (\<^bold>\<lambda>z. \<lparr>F,z,x,y\<rparr>) \<^bold>= (\<^bold>\<lambda>z. \<lparr>G,z,x,y\<rparr>)
+                      \<^bold>& (\<^bold>\<lambda>z. \<lparr>F,x,z,y\<rparr>) \<^bold>= (\<^bold>\<lambda>z. \<lparr>G,x,z,y\<rparr>)
+                      \<^bold>& (\<^bold>\<lambda>z. \<lparr>F,x,y,z\<rparr>) \<^bold>= (\<^bold>\<lambda>z. \<lparr>G,x,y,z\<rparr>)"
+  unfolding identity_\<Pi>\<^sub>3_def identity_\<Pi>\<^sub>1_def basic_identity\<^sub>3_def forall_\<kappa>_def by simp
 lemma identity\<^sub>\<o>_def[identity_defs]: "op \<^bold>= \<equiv> \<lambda>F G. (\<^bold>\<lambda>y. F) \<^bold>= (\<^bold>\<lambda>y. G)"
   unfolding identity_\<o>_def identity_\<Pi>\<^sub>1_def basic_identity\<^sub>\<o>_def by simp
 
